Goose leasing and dependencies

new/etc/update-goose-new.py
@@ -235,7 +235,12 @@ def main():
         "go.etcd.io/etcd/api/v3/mvccpb",
         "go.etcd.io/etcd/client/v3",
         "go.etcd.io/etcd/client/v3/concurrency",
-        "go.etcd.io/etcd/client/v3/concurrency",
+
+        "go.etcd.io/etcd/client/v3/leasing",
+        "go.etcd.io/etcd/api/v3/v3rpc/rpctypes",
+        "google.golang.org/grpc/codes",
+        "google.golang.org/grpc/status",
+
         "go.uber.org/zap",
         "go.uber.org/zap/zapcore",
     )
