new/proof/go_etcd_io/etcd/client/v3/leasing.v
@@ -1,0 +1,4 @@
+Require Import New.code.go_etcd_io.etcd.client.v3.leasing.
+Require Import New.generatedproof.go_etcd_io.etcd.client.v3.leasing.
+Require Import New.proof.proof_prelude.
+Require Import New.proof.context.
